added unflattening-function

theories/L/TM/TMflat.v
@@ -6,7 +6,7 @@ From PslBase.FiniteTypes Require Import VectorFin Cardinality.
 Inductive TM : Type :=
   { sig : nat;
     tapes : nat;
-    states : nat;      
+    states : nat;    
     trans : list ((nat * list (option nat)) * (nat * list (option nat * move)));
     start : nat;
     halt : list bool
@@ -16,10 +16,13 @@ Inductive isFlatteningTransOf {st sig : finType} {n}
           (f:list (nat * list (option nat) * (nat * list (option nat * move))))
           (f': st * Vector.t (option sig) n -> st * Vector.t (option sig * move) n): Prop :=
   mkIsFlatteningTransOf
-    (R__trans : forall s s' v v',
-        ((index s,map (option_map index) (Vector.to_list v))
-         ,(index s',map (map_fst (option_map index)) (Vector.to_list v'))) el f
-        <-> f' (s,v) = (s',v'))
+    (R__trans :
+       (forall s s' v v', ((s,v),(s',v')) el f <->
+       (exists s0 s0' v0 v0', f' (s0,v0) = (s0', v0')
+                         /\ s = index s0
+                         /\ s' = index s0'
+                         /\ v = map (option_map index) (Vector.to_list v0)
+                         /\ v' = map (map_fst (option_map index)) (Vector.to_list v0'))))
   : isFlatteningTransOf f f'.
 
 Inductive isFlatteningHaltOf {st:finType} (f : list bool) (f' : st -> bool) : Prop :=
@@ -32,7 +35,7 @@ Inductive isFlatteningTMOf {sig' n} (M:TM) (M': mTM sig' n) : Prop :=
   mkIsFlatteningTMOf
     (eq__tapes : tapes M = n)
     (eq__sig : sig M = Cardinality sig')
-    (eq__states : states M = Cardinality (TM.states M'))
+    (eq__states : (states M) = Cardinality (TM.states M'))
     (R__trans : isFlatteningTransOf (trans M) (TM.trans (m:=M')))
     (eq__start : start M = index (TM.start M'))
     (R__halt : isFlatteningHaltOf (halt M) (TM.halt (m:=M')))
@@ -47,100 +50,3 @@ Lemma isFlatteningTapesOf_iff (sig : finType) (n : nat) y (t:Vector.t (tape sig)
 Proof.
   split. now inversion 1. intros ->;easy.
 Qed.
-
-Notation "M '∼' M'" := (isFlatteningTMOf M M') (at level 60).
-
-
-(*
-Definition flatten_trans {states sig : finType} n
-           (f: states * Vector.t (option sig) n -> states * Vector.t (option sig * move) n) :  list (nat * list (option nat) * (nat * list (option nat * move)))
-  := map (fun '((st__i,l),(st__o,acts)) =>
-            ((index st__i,map (option_map index) (Vector.to_list l))
-             ,(index st__o,map (map_fst (option_map index)) (Vector.to_list acts)))) (finfunc_table f).
-
-Lemma test : (forall n m, n = m -> Fin.t n -> Fin.t m).
-  intros ? ? -> ?. assumption. Show Proof.
-Abort.
-
-Import Basics.
-Open Scope program_scope.
-
-Definition Vector_of_list_length A n (l:list A) : option (Vector.t A n) :=
-  match Nat.eq_dec (length l) n with
-    Specif.left H =>
-    Some (eq_rect _ (fun n => Vector.t A n) (Vector.of_list l) _ H)
-  | _ => None
-  end.
-
-Definition Fin_of_nat_try n i : option (Fin.t n) :=
-  match Fin.of_nat i n with
-    inleft x => Some x
-  | _ => None
-  end.
-
-Definition unflatten_symb sig  : nat -> option (Fin.t sig):=
-(Fin_of_nat_try sig).
-
-Fixpoint unflatten_acts' sig (l__r : list (option nat * move)): option (list (option (Fin.t sig) * move)) :=
-  match l__r with
-    nil => Some nil
-  | (i,m)::l__r =>
-    match unflatten_acts' sig l__r with
-    | None => None
-    | Some v__r => match option_map (unflatten_symb sig) i with
-                   Some None => None
-                 | None => Some ((None,m)::v__r)
-                 | Some i => Some ((i,m)::v__r)
-                 end
-    end
-  end.
-
-Definition unflatten_acts sig n (l__r : list (option nat * move)) : option (Vector.t (option (Fin.t sig)*move) n) :=
-  match unflatten_acts' sig l__r with
-    None => None
-  | Some l__r => Vector_of_list_length n l__r
-  end.
-  
-
-Definition unflatten_trans states sig n (f:list (nat * list (option nat) * (nat * list (option nat * move))))
-  : option (Fin.t states) * Vector.t (option (Fin.t sig)) n -> option (Fin.t states) * Vector.t (option (Fin.t sig) * move) n :=
-  fun '(st,l) =>
-    let d := (None,Vector.const (None,N) n) in
-    match st with
-    | Some st =>
-      let (st__o,l__r) := lookup f (index st,map (option_map ((@proj1_sig _ _ ) ∘ Fin.to_nat)) (Vector.to_list l)) (0,[]) in
-      match unflatten_acts sig n l__r with
-        None => d
-      | Some v=> 
-          (Fin_of_nat_try states st__o, v)
-      end
-    | _ => d
-    end.
-
-Definition flatten_halt {states : finType} (f: states -> bool) :
-  list bool
-  := map f (elem states).
-
-Definition unflatten_halt states (f: list bool) (i : option (Fin.t states)) : bool :=
-  match i with
-    None => false
-  | Some i => nth (proj1_sig (Fin.to_nat i)) f false
-  end.
-
-Definition from_mTM sig n (M:mTM sig n) : TM :=
-  {| sig := Cardinality sig ;
-     tapes := n;
-     states := Cardinality (TM.states M);
-     trans := flatten_trans (@TM.trans _ _ M);
-     start := index (TM.start M);
-     halt := flatten_halt (@TM.halt _ _ M);
-  |}.
-
-Definition to_mTM (M:TM) : mTM (finType_CS (Fin.t (sig M))) (tapes M) :=
-  {|TM.states := finType_CS (option (Fin.t (states M)));
-    TM.trans := unflatten_trans (trans M);
-    TM.start := Fin_of_nat_try _ (start M);
-    TM.halt := unflatten_halt (halt M);
-  |}.
-
-*)
