theories/L/TM/TMflatFun.v
@@ -23,6 +23,7 @@ Proof.
   all:nia.
 Qed.
 
+
 Lemma size_flatTapes (sig : finType) (n : nat) (t:list (tape nat)) (t' : Vector.t (tape sig) n):
   isFlatteningTapesOf t t'
   -> size (enc t) <= n * sizeOfmTapes t' * (Cardinality.Cardinality sig * 4 + 9) + n * 22 + 4.
@@ -38,4 +39,158 @@ Proof.
    cbn - [mult]. fold (Vector.to_list (Vector.map (mapTape index) x0)).
    specialize (IHn x0).
    rewrite size_flatTape. nia.
+Qed.
+
+
+
+Lemma sizeoftape_maptape_eq sig sig' (f:sig -> sig') t:
+  sizeOfTape (mapTape f t) = sizeOfTape t.
+Proof.
+  destruct t;cbn. all:repeat (cbn;simpl_list). all:lia.
+Qed.
+
+Fixpoint sizeOfmTapesFlat sig (ts : list (tape sig)) : nat :=
+  match ts with
+    [] => 0
+  | t::ts => max (sizeOfTape t) (sizeOfmTapesFlat ts)
+  end.
+
+Lemma sizeOfmTapesFlat_eq (sig : finType) (n : nat) (ts:list (tape nat)) (ts' : Vector.t (tape sig) n):
+  isFlatteningTapesOf ts ts'
+  -> sizeOfmTapesFlat ts = sizeOfmTapes ts'.
+Proof.
+  intro R__tapes. inv R__tapes. Set Printing Coercions.
+  unfold sizeOfmTapes,mapTapes.
+  rewrite Vector.fold_left_right_assoc_eq. 2:intros;nia.
+  induction n.
+  -rewrite !destruct_vector_nil with (v:=ts').
+   cbn. easy.
+  -edestruct destruct_vector_cons with (v:=ts') as (?&?&->).
+   cbn - [mult]. fold (Vector.to_list (Vector.map (mapTape index) x0)).
+   specialize (IHn x0). rewrite IHn,sizeoftape_maptape_eq. lia.
+Qed.
+
+Lemma isFlatteningTransOf_eq st sig' n trans trans' s v d:
+  isFlatteningTransOf (st:=st) (sig:=sig') (n:=n) trans trans' ->
+  (let (s',v'):= trans' (s,v) in
+  (index s', map (map_fst (option_map index)) (Vector.to_list v')))= lookup trans (index s,map (option_map index) (Vector.to_list v)) d.
+Proof.
+  intros [H].
+  destruct trans' as [s' v'] eqn:eq.
+  erewrite lookup_sound.
+  -reflexivity.
+  -intros [] [] []. rewrite !H.
+   intros (?&?&?&?&?&->&->&->&->).
+   intros (?&?&?&?&?&<-%injective_index&->&H'%map_injective&->).
+   2:{intros [] [] [=];f_equal. now eapply injective_index. }
+   eapply vector_to_list_inj in H' as <-.
+   congruence.
+  -rewrite H.
+   repeat eexists. easy.
+Qed.
+
+
+
+
+Print mconfig.
+Definition mconfigFlat :Type := nat * list (tape nat).
+
+Inductive isFlatteningConfigOf {st sig : finType} {n}: mconfigFlat -> mconfig st sig n -> Prop :=
+  mkisFlatteningConfigOf c c' (Hs : fst c = index c'.(cstate)) (Ht:isFlatteningTapesOf (snd c) c'.(ctapes))
+  : isFlatteningConfigOf c c'.
+Print step.
+
+Fixpoint zipWith {X Y Z} (f:X -> Y->Z) (xs:list X) (ys:list Y) : list Z :=
+  match xs,ys with
+    x::xs,y::ys => f x y :: zipWith f xs ys
+  | _,_ => []
+  end.
+
+Lemma doAct_multiFlat (sig:finType) n acts t (t' : tapes sig n):
+  isFlatteningTapesOf t t' ->
+  isFlatteningTapesOf (zipWith (doAct (sig:=nat)) t (map (map_fst (option_map index)) (Vector.to_list acts))) (doAct_multi t' acts).
+Proof.
+  intros H. inv H. rewrite isFlatteningTapesOf_iff.
+  induction n in *|-*.
+  -rewrite !destruct_vector_nil with (v:=t').
+   rewrite !destruct_vector_nil with (v:=acts). easy.
+  -destruct destruct_vector_cons with (v:=t') as (?&?&->).
+   destruct destruct_vector_cons with (v:=acts) as (?&?&->).
+   
+   cbn.
+   setoid_rewrite IHn.  f_equal.
+   destruct x,x1 as [[] []]; cbn - [tape_move_left tape_move_right]. all:try easy. 
+   all:try (setoid_rewrite <- mapTape_move_right || rewrite <- mapTape_move_left). all:cbn. all:easy.
+Qed.
+
+
+
+Definition stepFlat (trans:list (nat * list (option nat) * (nat * list (option nat * move)))) (c:mconfigFlat) : mconfigFlat :=
+  let (news, actions) := lookup trans (fst c, map (@current _) (snd c)) (0,[]) in (news,(zipWith (@doAct _) (snd c) actions)).
+
+Lemma current_charsFlat_eq (sig:finType) n t (t': tapes sig n):
+  isFlatteningTapesOf t t' ->
+  map (current (sig:=nat)) t = map ((option_map index)) (Vector.to_list (current_chars t')).
+Proof.
+  intros H. inv H. induction n in *|-*.
+  -rewrite !destruct_vector_nil with (v:=t'). easy.
+  -destruct destruct_vector_cons with (v:=t') as (?&?&->). cbn. setoid_rewrite IHn.
+   unfold current_chars. cbn.  f_equal.
+   destruct x; easy.
+Qed.
+
+Lemma stepFlat_eq sig' n (M': mTM sig' n) (trans:list (nat * list (option nat) * (nat * list (option nat * move)))) (c:mconfigFlat) c':
+  isFlatteningTransOf (sig:=sig') (n:=n) trans (TM.TM.trans (m:=M')) ->
+  isFlatteningConfigOf c c' -> 
+  isFlatteningConfigOf (stepFlat trans c) (step (M:=M') c').
+Proof.
+  intros Htrans H. inv H.
+  destruct c. cbn in Hs,Ht. inv Hs.
+
+  unfold stepFlat, step. cbn [fst snd cstate ctapes] in *.
+  erewrite current_charsFlat_eq. 2:easy.
+  erewrite <-isFlatteningTransOf_eq. 2:easy.
+  destruct TM.trans. econstructor. now easy.
+  cbn - [doAct_multi]. 
+  apply doAct_multiFlat. easy.
+Qed.
+
+Definition haltConfFlat (l : list bool) (c:mconfigFlat) : bool := nth (fst c) l false.  
+  
+Definition loopMflat M := loop (stepFlat M.(TMflat.trans)) (haltConfFlat M.(TMflat.halt)).
+
+Lemma loopMflat_correct (sig : finType) (n : nat) M (M' : mTM sig n)  k c c':
+  isFlatteningTMOf M M' ->
+  isFlatteningConfigOf c c' ->
+  match loopMflat M c k,loopM (M:=M') c' k with
+    None,None => True
+  | Some r,Some r' => isFlatteningConfigOf r r'
+  | _,_ => False
+  end.
+Proof.
+  intros HM Hc. unfold loopM,loopMflat.
+  induction k in Hc,c,c'|-*.
+  -cbn.
+   destruct HM. destruct R__halt. unfold haltConfFlat,haltConf.
+   inv Hc. destruct c. cbn in *. subst.
+   rewrite R__halt. destruct halt. 2:easy.
+   econstructor. all:easy.
+  -cbn.
+    destruct HM. destruct R__halt. unfold haltConfFlat,haltConf.
+   inversion Hc;subst. destruct c. cbn in *. subst.
+   rewrite R__halt. destruct halt. easy.
+   eapply stepFlat_eq in Hc. 2:eassumption. eapply IHk in Hc as H'.
+   fold (haltConfFlat (TMflat.halt M)). fold (haltConf (M:=M')). 
+   do 2 destruct loop. all:easy.
+Qed.
+
+Lemma initFlat_correct sig n M (M' : mTM sig n) t t':
+  isFlatteningTMOf M M' ->
+  isFlatteningTapesOf t t' ->
+  isFlatteningConfigOf (M.(TMflat.start), t) (initc M' t').
+Proof.
+  intros ? ?. inv H.
+  econstructor.
+  -easy.
+  -cbn. easy.
 Qed.
