theories/L/Complexity/Problems/TMGenericNPcompleteProblem.v
@@ -1,5 +1,5 @@
 From Undecidability.TM Require Import TM.
-From Undecidability.L.TM Require Import TMflatEnc TMEncoding TapeDecode.
+From Undecidability.L.TM Require Import TMflat TMflatEnc TMflatFun TMEncoding TapeDecode.
 From Undecidability.L.Datatypes Require Import LNat LProd Lists.
 
 
@@ -8,11 +8,10 @@ From Undecidability.L.Datatypes Require Import LNat LProd Lists.
 
 Definition TMgenericNPcompleteProblem: TM*nat*nat -> Prop:=
   fun '(M,maxSize, steps (*in unary*)) =>
-    exists sig n (M':mTM sig n), M ∼ M' /\ (exists t, (exists f, loopM (initc M' t) steps = Some f
-               /\ TM.halt (cstate f) = true)
+    exists sig n (M':mTM sig n), isFlatteningTMOf M M' /\ (exists t, (exists f, loopM (initc M' t) steps = Some f)
          /\ sizeOfmTapes t <= maxSize).
 
-
+ 
 From Undecidability.L.Complexity Require Import NP LinTimeDecodable.
 From Undecidability.L Require Import Tactics.LTactics Functions.Decoding TMflatFun.
 
@@ -22,16 +21,39 @@ Lemma inNP_TMgenericNPCompleteProblem:
   inNP TMgenericNPcompleteProblem.
 Proof.
   apply inNP_intro with (R:= fun '(M,maxSize, steps (*in unary*)) t =>
-                                exists sig n (M':mTM sig n) t', isFlatteningTapesOf t t' /\ M ∼ M' 
-                                       /\ (exists f, loopM (initc M' t') steps = Some f
-                                       /\ TM.halt (cstate f) = true)
-                                       /\ sizeOfmTapes t' <= maxSize).
+                               exists sig n (M':mTM sig n),
+                                 isFlatteningTMOf M M'
+                                 /\ exists t', isFlatteningTapesOf t t'
+                                         /\ (exists f, loopM (initc M' t') steps = Some f)
+                                         /\ sizeOfmTapes t' <= maxSize).
   now apply linDec_polyTimeComputable.
   -evar (f':nat -> nat).
    exists f'. repeat eapply conj.
    {
-     eexists (fun '((M,maxSize,steps),t) => _). repeat eapply conj.
-     2:{intros [[[TM maxSize] steps] y].  cbn. admit.
+     eexists (fun '((M,maxSize,steps),t) =>
+                if negb (sizeOfmTapesFlat t <=? maxSize)
+                then false
+                else match loopMflat M (M.(start),t) steps with
+                       Some _ => true
+                     | _ => false
+                     end).
+     repeat eapply conj.
+     2:{intros [[[M maxSize] steps] t]. cbn.
+        destruct (Nat.leb_spec0 (sizeOfmTapesFlat t) (maxSize));cbn [negb].
+        2:{ split. 2:easy.
+            intros (?&?&?&?&?&?&?&?). erewrite sizeOfmTapesFlat_eq in n. 2:easy. easy.
+        }
+        specialize loopMflat_correct with (M:=M) (c:=(M.(start),t)) (k:=steps) as H.
+        split.
+        -intros (?&?&M'&?&?&?&?&?).
+         specialize H with (1:=H0) (2:=initFlat_correct H0 H1).
+         destruct H2.
+         destruct loopMflat,loopM.
+         all:try easy.
+        -destruct loopMflat. 2:easy. intros _.
+         
+         
+        term+)
      }
      all:admit.
    }
