theories/L/TM/TMunflatten.v
@@ -1,0 +1,324 @@
+From Undecidability Require Import TM.TM L.Functions.FinTypeLookup.
+Require Import PslBase.FiniteTypes.
+From PslBase.FiniteTypes Require Import VectorFin Cardinality.
+
+From Undecidability Require Import L.TM.TMflat.
+
+
+Definition Vector_of_list_length A n (l:list A) : option (Vector.t A n) :=
+  match Nat.eq_dec (length l) n with
+    Specif.left H =>
+    Some (eq_rect _ (fun n => Vector.t A n) (Vector.of_list l) _ H)
+  | _ => None
+  end.
+
+Lemma Vector_of_list_length_eq A (l:list A) :
+  Vector_of_list_length (length l) l = Some (Vector.of_list l).
+Proof.
+  unfold Vector_of_list_length.
+  destruct _. 2:easy.
+  f_equal.
+  rewrite <- Eqdep_dec.eq_rect_eq_dec. easy. decide equality.
+Qed.
+(*
+Definition Fin_of_nat_try n i : option (Fin.t n) :=
+  match Fin.of_nat i n with
+    inleft x => Some x
+  | _ => None
+  end.*)
+
+Definition unflatten_symb (sig:finType)  (i:option nat): option sig:=
+  match i with
+    None => None
+  | Some i => nth i (map Some (elem _)) None
+  end.
+
+Definition unflatten_acts' (sig:finType) (l__r : list (option nat * move)): (list (option sig * move)) :=
+  map (fun '(i,m) => (unflatten_symb sig i,m)) l__r.
+
+Definition unflatten_acts (sig:finType) n (l__r : list (option nat * move)) : (Vector.t (option sig*move) n) :=
+  match Vector_of_list_length n  (unflatten_acts' sig l__r) with
+  | Some l__r => l__r
+  | _ => Vector.const (None,N) n
+  end.
+  
+
+Definition unflatten_trans (states:finType) (sig:finType) d n (f:list (nat * list (option nat) * (nat * list (option nat * move))))
+  : states * Vector.t (option sig) n -> states * Vector.t (option sig * move) n :=
+  fun '(st,l) =>
+    let (st__o,l__r) := lookup f (index st,map (option_map (fun x => index x)) (Vector.to_list l)) (0,[]) in
+    (nth st__o (elem _) d, unflatten_acts sig n l__r)
+.
+
+
+Definition unflatten_halt states (f: list bool) (i : (Fin.t states)) : bool :=
+  nth (index i) f false.
+(*
+Definition from_mTM sig n (M:mTM sig n) : TM :=
+  {| sig := Cardinality sig ;
+     tapes := n;
+     states := Cardinality (TM.states M);
+     trans := flatten_trans (@TM.trans _ _ M);
+     start := index (TM.start M);
+     halt := flatten_halt (@TM.halt _ _ M);
+  |}.*)
+
+Local Definition def n : Fin.t (max 1 n).
+Proof.
+  destruct n;cbn.
+  all:now constructor.
+Defined.
+
+Program Definition unflattenTM (M:TM) : mTM (finType_CS (Fin.t (sig M))) (tapes M) :=
+  let d := def _ in
+  {|TM.states := (finType_CS ((Fin.t (max 1 (states M)))));
+    TM.trans := unflatten_trans d (trans M);
+    TM.start := nth (start M) (elem _) d;
+    TM.halt := unflatten_halt (halt M);
+  |}.
+
+Lemma Card_Fint n : Cardinality (finType_CS (Fin.t n)) = n.
+Proof.
+Admitted.
+
+
+Lemma index_nth_elem (X:finType) i d:
+  i < Cardinality X
+  -> index (nth (A:=X) i (elem _) d) = i.
+Proof.
+  intros. unfold index. apply getPosition_nth.
+  -eapply dupfree_elements.
+  -refine (_:_ < Cardinality _). easy.
+Qed.
+
+Lemma index_nth_elem_fint i n d:
+  i < n
+  -> index (nth (A:=Fin.t n)i (elem _) d) = i.
+Proof.
+  intros. 
+  eapply index_nth_elem.
+  refine (_:_ < Cardinality _);setoid_rewrite Card_Fint at 1. easy.
+Qed.
+
+Definition defFin (X:finType):
+  0 < Cardinality X
+  -> X.
+Proof.
+  unfold Cardinality.
+  destruct (elem X). cbn. intros. omega. easy.
+Qed.
+  
+
+
+Definition unflatten_in (sig:finType) n (l__r : list (option nat)) : (Vector.t (option sig) n) :=
+  match Vector_of_list_length n  (map (unflatten_symb sig) l__r) with
+  | Some l__r => l__r
+  | _ => Vector.const None n
+  end.
+
+Lemma unflatten_in_correct (sig:finType) n v:
+  length v = n ->
+  (forall a : nat, Some a el v -> a < Cardinality sig) ->
+  map (option_map index) (Vector.to_list (unflatten_in sig n v)) = v.
+Proof.
+  intros <-.
+  unfold unflatten_in.
+  erewrite <- map_length.
+  rewrite Vector_of_list_length_eq,VectorSpec.to_list_of_list_opp.
+  rewrite utils.map_map_compose.
+  intros. 
+  erewrite map_ext_in with (g:=fun x => x). now apply map_id.
+  
+  intros. destruct a. 2:easy.
+  apply H in H0. 
+  unfold Basics.compose. cbn.
+  unshelve erewrite nth_indep with (d':= Some _).
+  -eapply defFin. omega.
+  -rewrite map_nth. cbn.
+   erewrite index_nth_elem. all:try easy.
+  -rewrite map_length. easy.
+Qed.
+
+Record validFlatTrans (states sig n:nat) (f:list (nat * list (option nat) * (nat * list (option nat * move)))) : Prop :=
+  {
+    flatTrans_inj:
+      (forall a' b1 b2 , (a', b1) el f -> (a', b2) el f -> b1 = b2);
+    flatTrans_tot:
+      (forall s v, (exists r, ((s,v),r) el f)  <-> s < states
+                                       /\ length v = n
+                                       /\ forall a, Some a el v -> a < sig);
+    flatTrans_res_ok: forall x s' v',
+        (x,(s',v')) el f
+        -> s' < states
+          /\ length v' = n
+          /\ (forall a m, (Some a,m) el v' -> a < sig)   
+  }.
+
+Lemma flatTrans_in_ok states sig n f:
+  validFlatTrans states sig n f ->
+  forall s v r,
+  ((s,v),r) el f
+  -> s < states
+    /\ length v = n
+    /\ (forall a, Some a el v -> a < sig).
+Proof.
+  intros H s v r ?.
+  eapply flatTrans_tot. all:eauto.
+Qed. 
+(*
+
+Lemma isFlattening_inv sig n (M':mTM sig n) d trans0 s s' v v':
+  isFlatteningTransOf trans0 (TM.trans (m:=M')) ->
+  ((s,v),(s',v')) el trans0 ->
+  s = index (nth s (elem (finType_CS (Fin.t (Cardinality (TM.states M'))))) d)
+  /\ s' = index (nth s' (elem (finType_CS (Fin.t (Cardinality (TM.states M'))))) d)
+  /\ v = map (option_map index) (unflatten_in (Cardinality sig) n v)
+  /\ v' = map (map_fst (option_map index)) (unflatten_acts (Cardinality sig) n v').
+Admitted.*)
+
+
+Lemma unflatten_acts_correct (sig:finType) n v':
+  length v' = n ->
+  (forall a m , (Some a,m) el v' -> a < Cardinality sig) ->
+  map (map_fst (option_map index)) (Vector.to_list (unflatten_acts sig n v')) = v'.
+Proof.
+  intros <-.
+  unfold unflatten_acts,unflatten_acts'.
+  erewrite <- map_length.
+  rewrite Vector_of_list_length_eq,VectorSpec.to_list_of_list_opp.
+  rewrite utils.map_map_compose.
+  intros. 
+  erewrite map_ext_in with (g:=fun x => x). now apply map_id.
+  
+  intros. destruct a as [[] ?]. 2:easy.
+  apply H in H0. 
+  unfold Basics.compose. cbn.
+  unshelve erewrite nth_indep with (d':= Some ltac:(eapply defFin)).
+  abstract omega.
+  2:{ rewrite map_length. easy. }
+
+  rewrite map_nth. cbn.
+  rewrite index_nth_elem;easy.
+Qed.
+
+Lemma vector_to_list_length X n (l: Vector.t X n):
+  length (Vector.to_list l) = n.
+Proof.
+  induction l;cbn. easy. rewrite IHl at 1. reflexivity.
+Qed.
+
+Lemma unflatten_trans_correct st sig n d trans0:
+  validFlatTrans st sig n trans0
+  -> isFlatteningTransOf trans0 (unflatten_trans (sig:=finType_CS (Fin.t sig)) (states := finType_CS (Fin.t st)) (n:=n) d trans0).
+Proof.
+  intros H.
+  econstructor;split.
+  -intros H'.
+   eexists (nth s (elem _) d),(nth s' (elem _) d).
+   eexists (unflatten_in _ _ v), (unflatten_acts _ _ v').
+   specialize (flatTrans_res_ok H H') as (?&?&?).
+   specialize (flatTrans_in_ok H H') as (?&?&?).
+   unfold unflatten_trans.
+   rewrite !index_nth_elem_fint. 2,3:easy.
+   rewrite unflatten_in_correct. 2,3:now try rewrite Card_Fint;easy.
+   erewrite lookup_sound. 3:easy. 2:eapply flatTrans_inj;eassumption.
+   cbn.
+   setoid_rewrite unflatten_in_correct. 2,3:now try rewrite Card_Fint;easy.
+   setoid_rewrite unflatten_acts_correct. 2,3:now try rewrite Card_Fint;easy.
+   repeat split.
+  -intros (?&?&?&?&H'&->&->&->&->).
+   unfold unflatten_trans in H'.
+   edestruct (proj2 (flatTrans_tot H (index x) (map (option_map index) (Vector.to_list x1) ))).
+   { repeat split.
+     -rewrite <- (Card_Fint). eapply index_le.
+     -clear. symmetry.  rewrite map_length,vector_to_list_length. reflexivity.
+     -intros ? ([]&[= <-]&?)%in_map_iff. rewrite <- (Card_Fint). eapply index_le.
+   }
+   erewrite lookup_sound in H'. 3:eassumption. 2:now eapply flatTrans_inj;eassumption.
+   destruct x3. inv H'.
+
+   specialize (flatTrans_res_ok H H0) as (?&?&?).
+   specialize (flatTrans_in_ok H H0) as (?&?&?).
+   
+   rewrite unflatten_acts_correct. 2,3:eauto.
+   rewrite index_nth_elem_fint. all:now try rewrite Card_Fint;easy.
+Qed.
+
+
+Lemma isFlatteningTrans_validFlatTrans n sig' (M' : mTM sig' n) f:
+isFlatteningTransOf f (TM.trans (m:=M'))
+-> validFlatTrans (Cardinality (TM.states M')) (Cardinality sig') n f.
+Proof.
+  intros [H'].
+  split.
+  -intros [] [] [] (?&?&?&?&?&->&->&->&->)%H' (?&?&?&?&?&eq1&->&eq2&->)%H'.
+   apply injective_index in eq1 as <-.
+   enough (x1=x5) by congruence.
+   clear - eq2.
+   eapply map_injective in eq2.
+   +now apply vector_to_list_inj.
+   +intros [] [] [=]. 2:easy.
+    f_equal;eauto using injective_index.
+  -intros. split.
+   +intros ([]&(?&?&?&?&?&->&->&->&->)%H').
+    repeat split.
+    *eapply index_le.
+    *rewrite map_length,vector_to_list_length. easy.
+    *intros ? ([]&[=<- ]&?)%in_map_iff. eapply index_le.
+   +intros (?&<-&?).
+    specialize H' with (s:=s) (v0:=v).
+    pose (s0 := nth s (elem (TM.states M')) (TM.start M')).
+    pose (v0 := unflatten_in sig' (length v) v).
+    destruct (TM.trans (s0,v0)) as (s0',v0') eqn:eq.
+    exists (index s0', map (map_fst (option_map index)) (Vector.to_list v0')). rewrite H'.
+    eexists _,s0',_,v0'.
+    repeat esplit.
+    *eassumption.
+    *subst s0. now erewrite index_nth_elem.
+    *subst v0. erewrite unflatten_in_correct. all:easy.
+  -intros [] ? ? (?&?&?&?&?&->&->&->&->)%H'.
+   rewrite map_length. repeat split.
+   +eapply index_le.
+   +apply vector_to_list_length.
+   +intros ? ? ([[]]&[= <- <-]&?)%in_map_iff. eapply index_le.
+Qed.
+
+Lemma unflattenTM_correct M:
+  (exists sig n (M' : mTM sig n), isFlatteningTMOf M M')
+  -> isFlatteningTMOf M (unflattenTM M).
+Proof.
+  intros (sig'&n&M'&H). destruct M. inv H.
+  assert (H_st:(Init.Nat.max 1 states) = states).
+  {destruct states. 2:easy.
+   exfalso.
+   enough (TM.start M' el []) by easy.
+   unfold Cardinality in eq__states.
+   symmetry in eq__states. eapply length_zero_iff_nil in eq__states.
+   rewrite <- eq__states.
+   eapply elem_spec.
+  }
+  cbn - [max] in *.
+  econstructor; cbn - [max].
+  -easy.
+  -now rewrite Card_Fint.
+  -cbn - [Cardinality max].
+   rewrite H_st.
+   setoid_rewrite <- Card_Fint at 1. easy.
+  -eapply unflatten_trans_correct. 
+   rewrite H_st. subst states sig.
+   eapply isFlatteningTrans_validFlatTrans. easy.
+  -cbn -[max].
+   generalize (def states).
+   rewrite H_st. intros ?.
+   unfold index. setoid_rewrite getPosition_nth. easy.
+   +apply dupfree_elements.
+   +rewrite eq__start, eq__states.
+    refine (_:_ < Cardinality _).
+    setoid_rewrite Card_Fint at 1.
+    unfold Cardinality.
+    eapply index_le.
+  -cbn -[max unflatten_trans]. rewrite H_st.
+   econstructor. reflexivity.
+Qed.
+
+Print Assumptions unflattenTM_correct.
